\lecture{Sept. 30}

\begin{exmp}
$$\{F\to (G\wedge H),(F\wedge G) \vee H\}\vDash H$$
\end{exmp}

\begin{proof}
Proof by contradiction. Suppose $H$ is false
\begin{align*}
   & (F\wedge G)\vee H , \neg H \quad \therefore F\wedge G\\
   & (F\wedge G) \quad \therefore F\\
   & F\to (G\wedge H) , F \quad \therefore G\wedge H\\
   & G\wedge H \quad \therefore H\\
   & \neg H , H \quad \textit{gives the contradiction} \\
   & \therefore H
\end{align*}
\end{proof}

Here is a derivation for the valid argument

\begin{tabular}{ll}
    $S = \{F\to (G\wedge H),(F\wedge G) \vee H, \neg H\} \vDash F\to (G\wedge H)$  & $\textit{ by V1 }$\\
    $S \vDash (F\wedge G) \vee H $ &$ \textit{ by V1 }$ \\
   $ S \vDash \neg H$  & $\textit{ V1 } $\\
    $S \vDash F\wedge G$  & $\textit{ V18 on line 2,3 }$ \\
   $ S \vDash F $ & $\textit{ V11 on line 4 }$ \\
   $ S \vDash G \wedge H $ & $\textit{ V23 on line 1,5 }$ \\
   $ S \vDash H $ & $\textit{ by V12 on 6 }$ \\
  $  \{F\to (G\wedge H),(F\wedge G) \vee H\} \vDash H$  & $\textit{ V5 on line 3,7 }$
\end{tabular}

Here is another proof 

\begin{proof}

Let $\alpha$ be an arbitrary assignment 

Suppose that $F\to (G\wedge H)$ is true (under $\alpha$)

Suppose that $(F\wedge G) \vee H$ is true

Note that wither $F\wedge G$ is true or $H$ is true

Case 1. Suppose $F\wedge G$ is true. [V14]

Since $F\wedge G$ $\therefore F$  [V11]

Since $F\to (G\wedge H)$ and $F$ $\therefore F$  [V23]

Since $G\wedge H$ $\therefore H$ [V12]

Case 2. Support that $H$ is true.  [V14]

Then $H$ is true.  [V1]

In either case, we have proven $H$ [V14]

\end{proof}


Here is a corresponding derivation of valid argument

\begin{enumerate}
    \item $S = \{F\to (G\wedge H),(F\wedge G)\} \vDash F \to (G\wedge H)$
    \item $S \vDash F\wedge G$
    \item $S\vDash F$
    \item $S\vDash G\wedge H$
    \item $S\vDash H$
    \item $\{F\to (G\wedge H),H\} \vDash H$
    \item $\{F\to (G\wedge H),(F\wedge G)\vee H\} \vDash H$
\end{enumerate}


\begin{exmp}
Show that 
\[
\{(F\vee \neg G) \to H, F\leftrightarrow (G\wedge \neg H)\}\vDash \neg (H\to F)
\]
\end{exmp}

\textbf{Solution: }We need to show that 

for every assignment $\alpha$

if $(F\vee \neg G) \to H$ is true under $\alpha$

and $F\leftrightarrow (G\wedge \neg H)$ is true

then $H\to F$ is false 

\begin{proof}
Let $\alpha$ be arbitrary assignment

Suppose $(F\vee \neg G) \to H$ is true

Suppose $F\leftrightarrow (G\wedge \neg H)$ is true.

[We need to show that $H\to F$ is false. Notice that $\neg (H\to F) \equiv H \wedge \neg F$. So we need to show that $H$ is true and $F$ is false.]

Suppose, for a contradiction, that $H$ is false.

Since $(F\vee \neg G) \to H$ and $\neg H \quad \therefore \neg(F\vee \neg G)$

Since $\neg (F\vee \neg G)\quad \therefore \neg F \wedge G$

Since $F\leftrightarrow (G\wedge \neg H)$ and $\neg F \quad \therefore \neg(G\wedge \neg H)$

Since $G$ and  $\neg H \quad \therefore G\wedge \neg H$

Since $G\wedge \neg H$ and $\neg (G\wedge \neg H)$ we have a contradiction

So $H$ is true.

Since $H$ is true, then $\neg \neg H$

Since $\neg \neg H$ we have $\neg G \vee \neg \neg H$

Since $\neg G \vee \neg \neg H$ we have $\neg (G\wedge \neg H)$

Since $F\leftrightarrow (G\wedge \neg H)$ and $\neg (G\wedge \neg H)$, we have $\neg F$

Since $H$ and $\neg F$, we have $H\wedge \neg F$

Since $H\wedge \neg F$ we have $\neg (H\to F)$


\end{proof}


\[
\{(F\vee \neg G) \to H, F\leftrightarrow (G\wedge \neg H)\}\vDash \neg (H\to F)
\]
Here is a derivation

\begin{proof}
\begin{enumerate}
    \item $S = \{(F\vee \neg G) \to H, F\leftrightarrow (G\wedge \neg H), \neg H\}\vDash \neg (H\to F)$  \hfill v1
    \item $S\vDash F \leftrightarrow (G\wedge \neg H)$ \hfill v1
    \item $S\vDash \neg H$ \hfill v1 
    \item $S\vDash \neg (F\vee \neg G)$ \hfill v24
    \item $S \vDash \neg F \wedge \neg \neg G$ \hfill v45,E8
    \item $S \vDash \neg F \wedge G $\hfill v11 on 5
    \item $S \vDash \neg F$ \hfill v31 on 2,6
    \item $S\vDash \neg \neg G$ \hfill 12 on 5
    \item $S\vDash G$ \hfill v45,e2 on 8
    \item $S\vDash G\wedge \neg H$ \hfill v10 on 9,3
    \item $T = \{(F\wedge \neg G)\to H,F\leftrightarrow(F\wedge\neg H)\} \vDash H$ \hfill v5 on 10,7
    \item $T \vDash \neg \neg H$
    \item $T \vDash \neg G \vee \neg \neg H$
    \item $T \vDash \neg (G\wedge \neg H)$
    \item $T \vDash F \leftrightarrow (G\wedge \neg H)$
    \item $T \vDash  \neg F$
    \item $T\vDash H\wedge \neg F$
    \item $T \vDash \neg (H\to F)$
\end{enumerate}
\end{proof}


