\lecture{Oct. 5}

\begin{exmp}
Find $\displaystyle \frac{3n^2+2n}{5n^2+2}$
\end{exmp}

\begin{solution}
\begin{align*}
    \lim_{n\to\infty} \frac{3n^2+2n}{5n^2+2}& = \lim_{n\to\infty} \frac{n^2}{n^2}\frac{3+\cfrac{2}{n}}{5+\cfrac{2}{n^2}}\\
    & = \frac{\displaystyle\lim_{n\to\infty} 3 + \lim_{n\to\infty} \cfrac{2}{n}}{\displaystyle\lim_{n\to\infty} 5 + \lim_{n\to\infty} \cfrac{2}{n^2}}\\
     & = \frac{3+0}{5+0} \\ 
     & = \frac{3}{5}
\end{align*}
\end{solution}

\begin{note}
If $a_kb_j\neq 0$
\begin{equation*}
    \lim_{n\to\infty} \frac{a_0+a_1n+\dots + a_kn^k}{b_0+b_1n+\dots + b_jn^j} = 
    \begin{cases}
        \displaystyle \frac{a_k}{b_j}  &  \textit{ if } k = j\\
        0 & \textit{ if } j>k\\
        \infty & \textit{ if } j<k, a_kb_j>0 \\
     -\infty & \textit{ if } j<k, a_kb_j<0 
    \end{cases}
\end{equation*}
\end{note}

\begin{exmp}
Find \[
\lim_{n\to\infty} \sqrt{n^2+n}-n\]
\end{exmp}

\begin{solution}
\begin{align*}
    \lim_{n\to\infty} \sqrt{n^2+n}-n &= 
    \lim_{n\to\infty} (\sqrt{n^2+n}-n)\cdot \frac{\sqrt{n^2+n}+n}{\sqrt{n^2+n}+n}\\
    & = \lim_{n\to\infty} \frac{n^2+n-n^2}{\sqrt{n^2+n}+n} \\
    & = \lim_{n\to\infty} \frac{n}{\sqrt{1+\cfrac{1}{n}}+1} \\ 
    & = \frac{n}{\sqrt{1+\displaystyle\lim_{n\to\infty}\frac{1}{n}}+1}\\
    & = \frac{1}{2}
\end{align*}
\end{solution}

\begin{exmp}
$a_1 = 1$ and $\displaystyle a_{n+1} = \frac{1}{1+a_n}$. Suppose that $\{a_n\}$ converges, find $\lim_{n\to \infty} a_n$
\end{exmp}

\begin{prop}
A sequence $\{a_n\}$ converges to $L$ if and only if every sub-sequence $\{a_{n_k}\}$ converges to L
\end{prop}
\begin{proof}
Assume that $lim_{n\to \infty} a_n = L$. Let $\{a_{n_k}\}$ be a sub-sequence. Let $\epsilon > 0$, we can find a $N_0$ so that if $n\geq N_0$, then $\abs{a_n - L}<\epsilon$.

Let $k_0 \geq N_0$, then $k\geq k_0 \Rightarrow n_k \geq n_{k_0}\geq N_0$

Hence $\abs{a_{n_k} - L}<\epsilon$
\end{proof}

\begin{solution}
If \[\lim_{n\to\infty} a_n = \lim_{n\to \infty} a_{n+1}\]

Then,
\begin{gather*}
    L = \frac{1}{1+L} \\
    L^2+L-1 = 0\\
    L = \frac{-1 \pm \sqrt{5}}{2}
\end{gather*}
\end{solution}

\begin{ques}
Does $\{a_n\}$ converge?
\end{ques}
\begin{solution}
Claim that for any k,
\[a_{2k}<a_{2k+2}<a_{2k+1}<a_{2k-1}\]
Proof by induction.

$\{a_{2k-1}\}$ is decreasing and bounded below by 0

$\{a_{2k}\}$ is increasing and bounded above by 1.

Let $\lim_{n\to\infty} a_{2k} = M$ and $\lim_{n\to\infty} a_{2k-1} = L$.

Since $M = \displaystyle \frac{-1 + \sqrt{5}}{2}$ and $L = \displaystyle \frac{-1 + \sqrt{5}}{2}$, $M = l$

Thus, $\{a_n\}$ converges.
\end{solution}
\begin{exmp}
FInd $$\lim_{n\to\infty} \frac{cos(n)}{n}$$
\end{exmp}



